transformations/Moore2Mealy/theorems/WFStable.v
@@ -17,7 +17,7 @@ Qed.
 
 Import Model Semantics.
 
-Lemma WF_transition_source_uniqueness_stable :
+Lemma transition_source_uniqueness_stable :
   forall m,
     Moore.WF_transition_source_exists m -> 
     MooreWF.WF_transition_source_uniqueness m -> 
@@ -40,5 +40,47 @@ Proof.
   reflexivity.
 Qed.
 
+Lemma transition_target_uniqueness_stable :
+  forall m,
+    MooreWF.WF_transition_target_uniqueness m -> 
+    MealyWF.WF_transition_target_uniqueness (Semantics.execute Moore2Mealy.Moore2Mealy m).
+Proof.
+  intros m WF4.
+  unfold MealyWF.WF_transition_target_uniqueness.
+  intros. 
+
+  destruct lk1 as (t' & s').
+  destruct lk2 as (t'' & s'').
+  simpl in H1. subst t''.
+  f_equal.
+  
+  destruct (Links.target_link_bw _ _ _ H) as (s1 & C1 & IN1).
+  destruct (Links.target_link_bw _ _ _ H0) as (s2 & C2 & IN2).
+
+  specialize (WF4 _ _ IN1 IN2 (eq_refl _)). 
+  PropUtils.inj WF4.
+  reflexivity.
+Qed.
+
 #[global]
-Hint Resolve WF_transition_source_uniqueness_stable : fw.
+Hint Resolve transition_source_uniqueness_stable transition_target_uniqueness_stable : wf.
+
+Lemma transition_target_glue_r_exists_stable m :
+  Moore.WF_transition_target_glue_r_exists m ->
+  Mealy.WF_transition_target_glue_r_exists (Semantics.execute Moore2Mealy.Moore2Mealy m).
+Proof.
+  unfold 
+    Moore.WF_transition_target_glue_r_exists, 
+    Mealy.WF_transition_target_glue_r_exists.
+  intros WF_MOORE t IN_MEALY.
+
+  destruct t.
+  apply Links.target_link_bw in IN_MEALY.
+  destruct IN_MEALY as (s0 & C & IN_MOORE).
+  unfold Glue.trg.
+  apply WF_MOORE in IN_MOORE.
+  unfold Glue.trg in IN_MOORE.
+  apply Elements.state_element_fw in IN_MOORE.
+  rewrite C in IN_MOORE.
+  exact IN_MOORE.
+Qed.
